C(sI-A)^{-1}B={\begin{pmatrix}2&1\cr \end{pmatrix}}{\begin{pmatrix}-1+s&15\cr -1&3+s\cr \end{pmatrix}}^{-1}{\begin{pmatrix}2\cr 0\cr \end{pmatrix}}={\begin{pmatrix}2&1\cr \end{pmatrix}}{\begin{pmatrix}{\frac{3+1s}{12+2s+s^{2}}}&{\frac{-15}{12+2s+s^{2}}}\cr {\frac{1}{12+2s+s^{2}}}&{\frac{-1+1s}{12+2s+s^{2}}}\cr \end{pmatrix}}{\begin{pmatrix}2\cr 0\cr \end{pmatrix}}={\begin{pmatrix}{\frac{7+2s}{12+2s+s^{2}}}&{\frac{-31+1s}{12+2s+s^{2}}}\cr \end{pmatrix}}{\begin{pmatrix}2\cr 0\cr \end{pmatrix}}={\dfrac{14+4s}{12+2s+s^{2}}}
